proof/correctproof/correct_get_addr_ofs.v
@@ -6,48 +6,51 @@ Require Import ZArith.
 
 From bpf.proof Require Import Clightlogic MatchState CorrectRel CommonLemma.
 
-From bpf.benchmark Require Import clightlogicexample.
+From bpf.clight Require Import interpreter.
+
 
 (**
-unsigned int get_add(unsigned int x, unsigned int y)
+unsigned int get_addr_ofs(unsigned long long x, int ofs)
 {
-  return x + y;
+  return (unsigned int) (x + (unsigned long long) ofs);
 }
 
-get_add = 
-fun x y : valu32_t => returnM (Val.add x y)
-     : valu32_t -> valu32_t -> M valu32_t
+Print get_addr_ofs.
+get_addr_ofs = 
+fun (x : val64_t) (ofs : sint32_t) =>
+returnM (val_intuoflongu (Val.addl x (Val.longofintu (sint32_to_vint ofs))))
+     : val64_t -> sint32_t -> M valu32_t
 
 *)
 
-Section Get_add.
+Section Get_addr_ofs.
 
   (** The program contains our function of interest [fn] *)
   Definition p : Clight.program := prog.
 
   (* [Args,Res] provides the mapping between the Coq and the C types *)
   (* Definition Args : list CompilableType := [stateCompilableType].*)
-  Definition args : list Type := [(valu32_t:Type); (valu32_t:Type)].
+  Definition args : list Type := [(val64_t:Type); (sint32_t:Type)].
   Definition res : Type := (valu32_t:Type).
 
   (* [f] is a Coq Monadic function with the right type *)
-  Definition f : arrow_type args (M res) := get_add.
+  Definition f : arrow_type args (M res) := get_addr_ofs.
 
   Variable state_block: block. (**r a block storing all rbpf state information? *)
 
   (* [fn] is the Cligth function which has the same behaviour as [f] *)
-  Definition fn: Clight.function := f_get_add.
+  Definition fn: Clight.function := f_get_addr_ofs.
 
   (* [match_arg] relates the Coq arguments and the C arguments *)
   Definition match_arg_list : DList.t (fun x => x -> val -> stateM -> Memory.Mem.mem -> Prop) args :=
-    (DList.DCons (stateless valu32_correct)
-       (DList.DCons (stateless valu32_correct)
+    (DList.DCons (stateless val64_correct)
+       (DList.DCons (stateless sint32_correct)
                     (DList.DNil _))).
 
   (* [match_res] relates the Coq result and the C result *)
   Definition match_res : res -> val -> stateM -> Memory.Mem.mem -> Prop := fun x v st m => valu32_correct x v.
 
-  Instance correct_function3_get_add : forall a, correct_function3 p args res f fn (nil) true match_arg_list match_res a.
+  Instance correct_function3_get_addr_ofs : forall a, correct_function3 p args res f fn (nil) true match_arg_list match_res a.
   Proof.
     correct_function_from_body args.
     correct_body.
@@ -56,22 +59,22 @@ Section Get_add.
     unfold f.
     repeat intro.
     get_invariant_more _x.
-    get_invariant_more _y.
+    get_invariant_more _ofs.
 
-    unfold stateless, valu32_correct in H1, H3.
+    unfold stateless, val64_correct in H1.
+    unfold stateless, sint32_correct in H3.
     destruct H1 as (Hc_eq & (vi & Hvi_eq)).
-    destruct H3 as (Hc0_eq & (vj & Hvj_eq)).
-    subst c c0 v v0.
+    subst c v v0.
 
-    (**according to the c function:
-unsigned int get_add(unsigned int x, unsigned int y)
+    (**according to the type of eval_pc:
+unsigned int get_addr_ofs(unsigned long long x, int ofs)
 {
-  return x + y;
+  return (unsigned int) (x + (unsigned long long) ofs);
 }
        1. return value should be  x+y
        2. the memory is same
       *)
-    exists (Val.add (Vint vi) (Vint vj)), m, Events.E0.
+    eexists. exists m, Events.E0.
 
     repeat split; unfold step2.
     -
@@ -83,6 +86,6 @@ unsigned int get_add(unsigned int x, unsigned int y)
       reflexivity.
   Qed.
 
-End Get_add.
+End Get_addr_ofs.
 
-Existing Instance correct_function3_get_add.
+Existing Instance correct_function3_get_addr_ofs.
