src/DxInstructions.v
@@ -13,7 +13,7 @@ Definition list_get (l: MyListType) (idx: sint32_t): M int64_t :=
   returnM (MyListIndexs32 l idx).
 
 Definition get_mem_region (n:nat): M memory_region :=
-  do mrs      <- eval_mem_regions;
+  do mrs      <- eval_mrs_regions;
   returnM (MyMemRegionsIndexnat mrs n).
 
 Definition get_dst (ins: int64_t): M reg :=
@@ -66,7 +66,7 @@ Definition get_sub (x y: valu32_t): M valu32_t := returnM (Val.sub x y).
 
 Definition get_addr_ofs (x: val64_t) (ofs: sint32_t): M valu32_t := returnM (val_intuoflongu (Val.addl x (Val.longofint (sint32_to_vint ofs)))).
 
-Definition get_block_ptr (mr: memory_region) : M valu32_t := returnM (block_ptr mr).
+Definition get_block_ptr (mr: memory_region) : M valptr32_t := returnM (block_ptr mr).
 
 Definition get_start_addr (mr: memory_region): M valu32_t := returnM (start_addr mr).
 
@@ -74,15 +74,13 @@ Definition get_block_size (mr: memory_region): M valu32_t := returnM (block_size
 
 Definition get_block_perm (mr: memory_region): M permission := returnM (block_perm mr).
 
-
-
 Definition is_well_chunk_bool (chunk: memory_chunk) : M bool :=
   match chunk with
   | Mint8unsigned | Mint16unsigned | Mint32 | Mint64 => returnM true
   | _ => returnM false
   end.
 
-Definition check_mem_aux2 (mr: memory_region) (addr: valu32_t) (chunk: memory_chunk): M valu32_t :=
+Definition check_mem_aux2 (mr: memory_region) (addr: valu32_t) (chunk: memory_chunk): M valptr32_t :=
   do well_chunk <- is_well_chunk_bool chunk;
     if well_chunk then
       do ptr    <- get_block_ptr mr;
@@ -95,21 +93,21 @@ Definition check_mem_aux2 (mr: memory_region) (addr: valu32_t) (chunk: memory_ch
                    (comp_eq_32 val32_zero (val32_modu lo_ofs (memory_chunk_to_valu32 chunk)))) then
             returnM (Val.add ptr lo_ofs) (**r > 0 *)
           else
-            returnM val32_zero (**r = 0 *)
+            returnM valptr_null (**r = 0 *)
         else
-          returnM val32_zero
+          returnM valptr_null
     else
-      returnM val32_zero.
+      returnM valptr_null.
 
-Fixpoint check_mem_aux (num: nat) (perm: permission) (chunk: memory_chunk) (addr: valu32_t) {struct num}: M valu32_t :=
+Fixpoint check_mem_aux (num: nat) (perm: permission) (chunk: memory_chunk) (addr: valu32_t) {struct num}: M valptr32_t :=
   match num with
-  | O => returnM val32_zero
+  | O => returnM valptr_null
   | S n =>
     do cur_mr   <- get_mem_region n;
     do mr_perm  <- get_block_perm cur_mr;
       if (perm_ge mr_perm perm) then
         do check_mem <- check_mem_aux2 cur_mr addr chunk;
-          if comp_eq_32 check_mem val32_zero then
+          if comp_eq_ptr32_zero check_mem then
             check_mem_aux n perm chunk addr
           else
             returnM check_mem
@@ -117,49 +115,17 @@ Fixpoint check_mem_aux (num: nat) (perm: permission) (chunk: memory_chunk) (addr
         check_mem_aux n perm chunk addr
   end.
 
-(*
-Definition check_mem_aux2 (mr: memory_region) (addr: valu32_t) (chunk: memory_chunk): M valu32_t :=
+Definition check_mem (perm: permission) (chunk: memory_chunk) (addr: valu32_t): M valptr32_t :=
   do well_chunk <- is_well_chunk_bool chunk;
     if well_chunk then
-      do lo_ofs <- get_sub addr (start_addr mr);
-      do hi_ofs <- get_add lo_ofs (memory_chunk_to_valu32 chunk);
-        if (andb (compu_le_32 val32_zero lo_ofs) (compu_lt_32 hi_ofs (block_size mr))) then
-          if (andb (compu_le_32 lo_ofs (memory_chunk_to_valu32_upbound chunk))
-                   (comp_eq_32 val32_zero (val32_modu lo_ofs (memory_chunk_to_valu32 chunk)))) then
-            returnM (Val.add (block_ptr mr) lo_ofs) (**r > 0 *)
-          else
-            returnM val32_zero (**r = 0 *)
-        else
-          returnM val32_zero
-    else
-      returnM val32_zero.
-
-Fixpoint check_mem_aux (num: nat) (perm: permission) (chunk: memory_chunk) (addr: valu32_t) {struct num}: M valu32_t :=
-  match num with
-  | O => returnM val32_zero
-  | S n =>
-    do cur_mr <- get_mem_region n;
-      if (perm_ge (block_perm cur_mr) perm) then
-        do check_mem <- check_mem_aux2 cur_mr addr chunk;
-          if comp_eq_32 check_mem val32_zero then
-            check_mem_aux n perm chunk addr
-          else
-            returnM check_mem
-      else
-        check_mem_aux n perm chunk addr
-  end. *)
-
-Definition check_mem (perm: permission) (chunk: memory_chunk) (addr: valu32_t): M valu32_t :=
-  do well_chunk <- is_well_chunk_bool chunk;
-    if well_chunk then
-      do mem_reg_num <- eval_mem_num;
+      do mem_reg_num <- eval_mrs_num;
       do check_mem <- check_mem_aux mem_reg_num perm chunk addr;
-        if comp_eq_32 check_mem val32_zero then
-          returnM val32_zero
+        if comp_eq_ptr32_zero check_mem then
+          returnM valptr_null
         else
           returnM check_mem
     else
-      returnM val32_zero.
+      returnM valptr_null.
 
 Definition comp_and_0x08_byte (x: int8_t): M bool :=  returnM (Byte.eq int8_zero (Byte.and x int8_0x08)).
 
@@ -387,7 +353,7 @@ Definition step_opcode_mem_ld_reg (addr: valu32_t) (pc: sint32_t) (dst: reg) (op
   match opcode_ld with
   | op_BPF_LDXW      =>
     do addr_ptr <- check_mem Readable Mint32 addr;
-      if comp_eq_32 addr_ptr val32_zero then
+      if comp_eq_ptr32_zero addr_ptr then
         upd_flag BPF_ILLEGAL_MEM
       else
         do v <- load_mem Mint32 addr_ptr;
@@ -395,7 +361,7 @@ Definition step_opcode_mem_ld_reg (addr: valu32_t) (pc: sint32_t) (dst: reg) (op
           upd_flag BPF_OK
   | op_BPF_LDXH      =>
     do addr_ptr <- check_mem Readable Mint16unsigned addr;
-      if comp_eq_32 addr_ptr val32_zero then
+      if comp_eq_ptr32_zero addr_ptr then
         upd_flag BPF_ILLEGAL_MEM
       else
         do v <- load_mem Mint16unsigned addr_ptr;
@@ -403,7 +369,7 @@ Definition step_opcode_mem_ld_reg (addr: valu32_t) (pc: sint32_t) (dst: reg) (op
           upd_flag BPF_OK
   | op_BPF_LDXB      =>
     do addr_ptr <- check_mem Readable Mint8unsigned addr;
-      if comp_eq_32 addr_ptr val32_zero then
+      if comp_eq_ptr32_zero addr_ptr then
         upd_flag BPF_ILLEGAL_MEM
       else
         do v <- load_mem Mint8unsigned addr_ptr;
@@ -411,7 +377,7 @@ Definition step_opcode_mem_ld_reg (addr: valu32_t) (pc: sint32_t) (dst: reg) (op
           upd_flag BPF_OK
   | op_BPF_LDXDW     =>
     do addr_ptr <- check_mem Readable Mint64 addr;
-      if comp_eq_32 addr_ptr val32_zero then
+      if comp_eq_ptr32_zero addr_ptr then
         upd_flag BPF_ILLEGAL_MEM
       else
         do v <- load_mem Mint64 addr_ptr;
@@ -425,28 +391,28 @@ Definition step_opcode_mem_st_imm (imm: vals32_t) (addr: valu32_t) (pc: sint32_t
   match opcode_st with
   | op_BPF_STW       =>
     do addr_ptr <- check_mem Writable Mint32 addr;
-      if comp_eq_32 addr_ptr val32_zero then
+      if comp_eq_ptr32_zero addr_ptr then
         upd_flag BPF_ILLEGAL_MEM
       else
         do _ <- store_mem_imm Mint32 addr_ptr imm;
           upd_flag BPF_OK
   | op_BPF_STH       =>
     do addr_ptr <- check_mem Writable Mint16unsigned addr;
-      if comp_eq_32 addr_ptr val32_zero then
+      if comp_eq_ptr32_zero addr_ptr then
         upd_flag BPF_ILLEGAL_MEM
       else
         do _ <- store_mem_imm Mint16unsigned addr_ptr imm;
           upd_flag BPF_OK
   | op_BPF_STB       =>
     do addr_ptr <- check_mem Writable Mint8unsigned addr;
-      if comp_eq_32 addr_ptr val32_zero then
+      if comp_eq_ptr32_zero addr_ptr then
         upd_flag BPF_ILLEGAL_MEM
       else
         do _ <- store_mem_imm Mint8unsigned addr_ptr imm;
           upd_flag BPF_OK
   | op_BPF_STDW      =>
     do addr_ptr <- check_mem Writable Mint64 addr;
-      if comp_eq_32 addr_ptr val32_zero then
+      if comp_eq_ptr32_zero addr_ptr then
         upd_flag BPF_ILLEGAL_MEM
       else
         do _ <- store_mem_imm Mint64 addr_ptr imm;
@@ -459,28 +425,28 @@ Definition step_opcode_mem_st_reg (src64: val64_t) (addr: valu32_t) (pc: sint32_
   match opcode_st with
   | op_BPF_STXW      =>
     do addr_ptr <- check_mem Writable Mint32 addr;
-      if comp_eq_32 addr_ptr val32_zero then
+      if comp_eq_ptr32_zero addr_ptr then
         upd_flag BPF_ILLEGAL_MEM
       else
         do _ <- store_mem_reg Mint32 addr_ptr src64;
           upd_flag BPF_OK
   | op_BPF_STXH      =>
     do addr_ptr <- check_mem Writable Mint16unsigned addr;
-      if comp_eq_32 addr_ptr val32_zero then
+      if comp_eq_ptr32_zero addr_ptr then
         upd_flag BPF_ILLEGAL_MEM
       else
         do _ <- store_mem_reg Mint16unsigned addr_ptr src64;
           upd_flag BPF_OK
   | op_BPF_STXB      =>
     do addr_ptr <- check_mem Writable Mint8unsigned addr;
-      if comp_eq_32 addr_ptr val32_zero then
+      if comp_eq_ptr32_zero addr_ptr then
         upd_flag BPF_ILLEGAL_MEM
       else
         do _ <- store_mem_reg Mint8unsigned addr_ptr src64;
           upd_flag BPF_OK
   | op_BPF_STXDW     =>
     do addr_ptr <- check_mem Writable Mint64 addr;
-      if comp_eq_32 addr_ptr val32_zero then
+      if comp_eq_ptr32_zero addr_ptr then
         upd_flag BPF_ILLEGAL_MEM
       else
         do _ <- store_mem_reg Mint64 addr_ptr src64;
