proof/CommonLib.v
@@ -1,0 +1,47 @@
+From bpf.src Require Import DxIntegers DxValues DxAST DxRegs DxFlag.
+From compcert Require Import Integers.
+From Coq Require Import ZArith.
+Open Scope Z_scope.
+
+(** common libs for clightlogic
+
+*)
+
+Definition id_of_reg (r:reg) : Z :=
+  match r with
+  | R0 => 0
+  | R1 => 1
+  | R2 => 2
+  | R3 => 3
+  | R4 => 4
+  | R5 => 5
+  | R6 => 6
+  | R7 => 7
+  | R8 => 8
+  | R9 => 9
+  | R10 => 10
+  end.
+
+Definition Z_of_flag (f:bpf_flag) : Z :=
+  match f with
+  | BPF_SUCC_RETURN  => 1
+  | BPF_OK  => 0
+  | BPF_ILLEGAL_INSTRUCTION => -1
+  | BPF_ILLEGAL_MEM => -2
+  | BPF_ILLEGAL_JUMP => -3
+  | BPF_ILLEGAL_CALL => -4
+  | BPF_ILLEGAL_LEN  => -5
+  | BPF_ILLEGAL_REGISTER => -6
+  | BPF_NO_RETURN => -7
+  | BPF_OUT_OF_BRANCHES => -8
+  | BPF_ILLEGAL_DIV => -9
+  | BPF_ILLEGAL_SHIFT => -10
+  | BPF_ILLEGAL_ALU => -11
+  | BPF_UNDEF_ERROR => -12
+  end.
+
+Definition int_of_flag (f:bpf_flag)  :=
+  Int.repr (Z_of_flag f).
+
+
+Close Scope Z_scope.
