proof/correctproof/correct_get_opcode_alu64.v
@@ -1,0 +1,85 @@
+From bpf.src Require Import DxIntegers DxValues DxOpcode DxMemRegion DxState DxMonad DxInstructions.
+From Coq Require Import List Lia ZArith.
+From compcert Require Import Integers Values Clight Memory.
+Import ListNotations.
+
+From bpf.proof Require Import Clightlogic MatchState CorrectRel CommonLemma.
+
+From bpf.clight Require Import interpreter.
+
+
+(**
+Check get_opcode_alu64.
+get_opcode_alu64
+     : int8_t -> M DxOpcode.opcode_alu64
+
+*)
+
+Section Get_opcode_alu64.
+
+  (** The program contains our function of interest [fn] *)
+  Definition p : Clight.program := prog.
+
+  (* [Args,Res] provides the mapping between the Coq and the C types *)
+  (* Definition Args : list CompilableType := [stateCompilableType].*)
+  Definition args : list Type := [(int8_t:Type)].
+  Definition res : Type := (opcode_alu64:Type).
+
+  (* [f] is a Coq Monadic function with the right type *)
+  Definition f : arrow_type args (M res) := get_opcode_alu64.
+
+  Variable state_block: block. (**r a block storing all rbpf state information? *)
+
+  (* [fn] is the Cligth function which has the same behaviour as [f] *)
+  Definition fn: Clight.function := f_get_opcode_alu64.
+
+  (* [match_arg] relates the Coq arguments and the C arguments *)
+  Definition match_arg_list : DList.t (fun x => x -> val -> stateM -> Memory.Mem.mem -> Prop) args :=
+    (DList.DCons (stateless int8_correct)
+                (DList.DNil _)).
+
+  (* [match_res] relates the Coq result and the C result *)
+  Definition match_res : res -> val -> stateM -> Memory.Mem.mem -> Prop := fun x v st m => opcode_alu64_correct x v.
+
+  Instance correct_function3_get_opcode_alu64 : forall a, correct_function3 p args res f fn nil true match_arg_list match_res a.
+  Proof.
+    correct_function_from_body args.
+    correct_body.
+    (** how to use correct_* *)
+    unfold INV.
+    unfold f.
+    repeat intro.
+    get_invariant_more _op.
+
+    unfold stateless, int8_correct in H1.
+    subst.
+
+    eexists. exists m, Events.E0.
+
+    repeat split; unfold step2.
+    -
+      repeat forward_star.
+    - simpl.
+      (**r Search (Int.zero_ext).*)
+      rewrite Int.zero_ext_idem;[idtac | lia].
+      unfold match_res, opcode_alu64_correct, byte_to_opcode_alu64.
+      match goal with
+      | |- (match ?X with | _ => _ end) =>
+          destruct X; eexists; reflexivity
+      end.
+    - simpl.
+      constructor.
+      rewrite Int.zero_ext_idem;[idtac | lia].
+      simpl.
+      rewrite Int.zero_ext_idem;[idtac | lia].
+      reflexivity. (*
+    - unfold unmodifies_effect.
+      intros.
+      destruct modifies.
+      reflexivity.
+      intros; reflexivity.*)
+  Qed.
+
+End Get_opcode_alu64.
+
+Existing Instance correct_function3_get_opcode_alu64.
