proof/correctproof/correct_is_well_chunk_bool.v
@@ -40,8 +40,8 @@ Ltac exec_seq_of_labeled_statement :=
       change (seq_of_labeled_statement X) with x
   end.
 
-Instance correct_function_is_well_chunk_bool2 : forall unmod a, correct_function3
-    p args res f fn unmod true (DList.DCons  (stateless match_chunk) (DList.DNil _)) (stateless match_bool) a.
+Instance correct_function_is_well_chunk_bool2 : forall a, correct_function3
+    p args res f fn nil true (DList.DCons  (stateless match_chunk) (DList.DNil _)) (stateless match_bool) a.
 Proof.
   correct_function_from_body args.
   correct_body.
@@ -72,6 +72,8 @@ Proof.
   - simpl.
     constructor.
     destruct v' ; reflexivity.
+  - unfold is_well_chunk_bool, returnM in Heq.
+    destruct c; inversion Heq; reflexivity.
 Qed.
 
 (*
