proof/correctproof/correct_step_opcode_alu64.v
@@ -1,0 +1,228 @@
+From bpf.src Require Import DxIntegers DxValues DxOpcode DxMemRegion DxRegs DxState DxMonad DxInstructions.
+From Coq Require Import List Lia ZArith.
+From compcert Require Import Integers Values Clight Memory.
+Import ListNotations.
+
+From bpf.proof Require Import Clightlogic MatchState CorrectRel CommonLemma.
+
+From bpf.clight Require Import interpreter.
+
+From bpf.proof.correctproof Require Import correct_get_opcode_alu64.
+(**
+Check step_opcode_alu64.
+step_opcode_alu64
+     : val64_t -> val64_t -> DxRegs.reg -> int8_t -> M unit
+
+*)
+
+Section Step_opcode_alu64.
+
+  (** The program contains our function of interest [fn] *)
+  Definition p : Clight.program := prog.
+
+  (* [Args,Res] provides the mapping between the Coq and the C types *)
+  (* Definition Args : list CompilableType := [stateCompilableType].*)
+  Definition args : list Type := [(val64_t:Type); (val64_t:Type); (reg:Type); (int8_t:Type)].
+  Definition res : Type := unit.
+
+  (* [f] is a Coq Monadic function with the right type *)
+  Definition f : arrow_type args (M res) := step_opcode_alu64.
+
+  Variable state_block: block. (**r a block storing all rbpf state information? *)
+
+  Definition modifies : list block := [state_block]. (* of the C code *)
+
+  Definition stateM_correct (st:unit) (v: val) (stm:stateM) (m: Memory.Mem.mem) :=
+    v = Vptr state_block Ptrofs.zero /\ match_state state_block stm m.
+
+  (* [fn] is the Cligth function which has the same behaviour as [f] *)
+  Definition fn: Clight.function := f_step_opcode_alu64.
+
+  (* [match_arg] relates the Coq arguments and the C arguments *)
+  Definition match_arg_list : DList.t (fun x => x -> val -> stateM -> Memory.Mem.mem -> Prop) ((unit:Type) ::args) :=
+    (DList.DCons stateM_correct
+      (DList.DCons (stateless val64_correct)
+       (DList.DCons (stateless val64_correct)
+          (DList.DCons (stateless reg_correct)
+            (DList.DCons (stateless int8_correct)
+                    (DList.DNil _)))))).
+
+  (* [match_res] relates the Coq result and the C result *)
+  Definition match_res : res -> val -> stateM -> Memory.Mem.mem -> Prop := fun x v st m => True.
+
+
+Ltac build_app_aux T :=
+  match T with
+  | ?F ?X => let ty := type of X in
+             let r := build_app_aux F in
+             constr:((mk ty X) :: r)
+  | ?X    => constr:(@nil dpair)
+  end.                                    
+
+Ltac get_function T :=
+  match T with
+  | ?F ?X => get_function F
+  | ?X    => X
+  end.
+
+Ltac build_app T :=
+  let a := build_app_aux T in
+  let v := (eval simpl in (DList.of_list_dp (List.rev a))) in
+  let f := get_function T in
+  match type of v with
+  | DList.t _ ?L =>
+      change T with (app (f: arrow_type L _) v)
+  end.
+
+Ltac change_app_for_body :=
+  match goal with
+  | |- @correct_body _ _ ?F _ _ _ _ _ _ _ _
+    => build_app F
+  end.
+
+Ltac change_app_for_statement :=
+  match goal with
+  | |- @correct_statement _ _ ?F _ _ _ _ _ _ _ _
+    => build_app F
+  end.
+
+Ltac prove_incl :=
+  simpl; unfold incl; simpl; intuition congruence.
+
+Ltac prove_in_inv :=
+  simpl; intuition subst; discriminate.
+
+Ltac correct_forward L :=
+  match goal with
+  | |- @correct_body _ _ (bindM ?F1 ?F2)  _
+                     (Ssequence
+                        (Ssequence
+                           (Scall _ _ _)
+                           (Sset ?V ?T))
+                        ?R)
+                     _ _ _ _ _ _  =>
+      eapply L;
+      [ change_app_for_statement ;
+        let b := match T with
+                 | Ecast _ _ => constr:(true)
+                 | _         => constr:(false)
+                 end in
+        eapply correct_statement_call with (has_cast := b)
+      |]
+  | |- @correct_body _ _ (match  ?x with true => _ | false => _ end) _
+                     (Sifthenelse _ _ _)
+                     _ _ _ _ _ _  =>
+      eapply correct_statement_if_body; [prove_in_inv | destruct x ]
+  end.
+
+  Instance correct_function3_step_opcode_alu64 : forall a, correct_function3 p args res f fn modifies false match_arg_list match_res a.
+  Proof.
+    correct_function_from_body args.
+    correct_body.
+
+    unfold f, step_opcode_alu64.
+    simpl.
+    (** goal: correct_body _ _ (bindM (get_opcode_alu64 _) ... *)
+    correct_forward correct_statement_seq_body_nil.
+
+    reflexivity.
+    reflexivity.
+    reflexivity.
+    typeclasses eauto.
+
+    { unfold INV.
+      unfold var_inv_preserve. (**r unmodifies_effect is not enough, we also need unmodifies_effect_state *)
+      intros.
+      unfold match_temp_env in *.
+      rewrite Forall_fold_right in *.
+      simpl in *.
+      destruct H; subst.
+      intuition.
+    }
+
+    reflexivity.
+    reflexivity.
+    reflexivity.
+    prove_in_inv.
+    prove_in_inv.
+    reflexivity.
+    reflexivity.
+
+    intros.
+    change (match_temp_env INV le st m) in H; unfold INV in H.
+    get_invariant _op.
+    exists (v::nil).
+    split.
+    unfold map_opt. unfold exec_expr. rewrite p0.
+    reflexivity.
+    intros. simpl.
+    tauto.
+
+    (** goal: correct_body _ _
+              match x with
+              | op_BPF_ADD64 => bindM (upd_reg ... *)
+    intros.
+    unfold INV.
+    destruct x. (**r case discussion on each alu64_instruction *)
+    - (**r op_BPF_ADD64 *)
+      unfold correct_body.
+      intros.
+      correct_forward correct_statement_seq_body.
+    - (**r op_BPF_SUB64 *)
+    - (**r op_BPF_MUL64 *)
+    - (**r op_BPF_DIV64 *)
+    - (**r op_BPF_OR64 *)
+    - (**r op_BPF_AND64 *)
+    - (**r op_BPF_LSH64 *)
+    - (**r op_BPF_RSH64 *)
+    - (**r op_BPF_NEG64 *)
+    - (**r op_BPF_MOD64 *)
+    - (**r op_BPF_XOR64 *)
+    - (**r op_BPF_ARSH64 *)
+    - (**r op_BPF_ALU64_ILLEGAL_INS *)
+    unfold f, step_opcode_alu64.
+    repeat intro.
+    match goal with
+    | |- match ?X with | _ => _  end =>
+      destruct X eqn: Hx; [ idtac | constructor]
+    end.
+    destruct p0.
+    intros.
+
+    get_invariant_more _st.
+    get_invariant_more _src64.
+    get_invariant_more _dst.
+    get_invariant_more _op.
+    unfold stateM_correct in H1.
+    destruct H1 as (H1_eq & H1_st).
+    destruct H1_st.
+    unfold stateless, val64_correct in H3.
+    destruct H3 as (H3_eq & (H3_vl & H3_c0)).
+    unfold stateless, reg_correct in H5.
+    unfold stateless, int8_correct in H7.
+    subst.
+
+    do 2 eexists; exists Events.E0.
+
+    repeat split; unfold step2.
+    -
+      forward_star.
+      repeat forward_star.
+      forward_star.
+      repeat forward_star.
+      
+      forward_star.
+      repeat forward_star.
+      
+      forward_star.
+      repeat forward_star.
+    - simpl.
+      eexists; reflexivity.
+    - simpl.
+      constructor.
+      reflexivity.
+  Qed.
+
+End Step_opcode_alu64.
+
+Existing Instance correct_function3_step_opcode_alu64.
